compiler/backend/proofs/stack_to_labProofScript.sml
@@ -1818,7 +1818,7 @@ val full_make_init_semantics = save_thm("full_make_init_semantics",let
 val full_make_init_semantics_fail = save_thm("full_make_init_semantics_fail",let
   val th = from_remove_fail |> DISCH_ALL |> REWRITE_RULE lemmas
            |> GEN_ALL |> SIMP_RULE (srw_ss()) [] |> SPEC_ALL
-           |> Q.INST [`code3`|->`compile c code4`] |> REWRITE_RULE []
+           |> Q.INST [`code3`|->`stack_alloc$compile c code4`] |> REWRITE_RULE []
            |> Q.INST [`code1`|->`compile max_heap bitmaps k start (compile c code4)`]
            |> REWRITE_RULE (AND_IMP_INTRO::GSYM CONJ_ASSOC::lemmas)
            |> Q.INST [`code4`|->`code`]
